Rope/Basic.lean
@@ -11,15 +11,13 @@ def Row : Type := Quotient WF.Row.instSetoid
 
 def Ty : Type := Quotient WF.Ty.instSetoid
 
-instance : LE Row where
-  le :=
-    Quotient.lift₂ WF.Row.le <| by
-      intro a1 b1 a2 b2 aeq beq
-      cases aeq; cases beq;
-      case _ ha hb =>
-        
-        
-        sorry
+-- instance : LE Row where
+--   le :=
+--     Quotient.lift₂ WF.Row.le <| by
+--       intro a1 b1 a2 b2 aeq beq
+--       cases aeq; cases beq;
+--       case _ ha1 ha2 hb1 hb2 =>
+--         sorry
 
 -- def lack (r1 r2 : Row) : Prop :=
 --   Quotient.lift WF.lack <| by
